theories/opt/ex3.v
@@ -4,32 +4,36 @@ Set Default Proof Using "Type".
 
 (** Moving a write to a mutable reference up across unknown code. *)
 
+(* TODO: check if Free is in the right place *)
 (* Assuming x : &mut i32 *)
 Definition ex3 : function :=
   fun: ["i"],
     let: "x" := new_place (&mut int) "i" in
-    Retag "x"  FnEntry ;;
+    retag_place "x" (RefPtr Mutable) int FnEntry ;;
     *{int} "x" <- #[42] ;;
     let: "v" := Call #[ScFnPtr "f"] [] in
     *{int} "x" <- #[13] ;;
+    Free "x" ;; Free "i" ;;
     "v"
   .
 
 Definition ex3_opt_1 : function :=
   fun: ["i"],
     let: "x" := new_place (&mut int) "i" in
-    Retag "x"  FnEntry ;;
+    retag_place "x" (RefPtr Mutable) int FnEntry ;;
     *{int} "x" <- #[42] ;;
     *{int} "x" <- #[13] ;;
-    Call #[ScFnPtr "f"] []
+    Call #[ScFnPtr "f"] [] ;;
+    Free "x" ;; Free "i"
   .
 
 Definition ex3_opt_2 : function :=
   fun: ["i"],
     let: "x" := new_place (&mut int) "i" in
-    Retag "x"  FnEntry ;;
+    retag_place "x" (RefPtr Mutable) int FnEntry ;;
     *{int} "x" <- #[13] ;;
-    Call #[ScFnPtr "f"] []
+    Call #[ScFnPtr "f"] [] ;;
+    Free "x" ;; Free "i"
   .
 
 Lemma ex3_sim_fun : ⊨ᶠ ex3 ≥ ex3_opt_1.
